Define <= for labels using lub

fstar/Label.fst
@@ -4,17 +4,11 @@ type label =
  | Low : label
  | High : label
 
-(*
-val op_Less : label -> label -> bool
-let op_Less l1 l2 = match l1, l2 with
- | Low, High -> true
- | _, _ -> false
-
-val op_Less_Equals : label -> label -> bool
-let op_Less_Equals l1 l2 = l1 < l2 || l1 = l2
-*)
 
 val lub : label -> label -> label
 let lub l1 l2 = match l1, l2 with
  | Low, Low -> Low
  | _, _ -> High
+
+val leq : label -> label -> bool
+let leq l1 l2 = lub l1 l2 = l2
